exercises.v
@@ -9,7 +9,7 @@ Definition ex_123_permutation: permutation 5.
 Proof.
   refine (let H := (_: permutation_list 5) in plist_to_permutation H).
   pose (1::2::4::3::0::nil) as L. exists L. pose (aux3_reflect 5 L).
-  simpl in *. inversion r. auto.
+  inversion r. auto.
 Defined.
 Eval compute in show ex_123_permutation.
 Eval compute in count_inversions ex_123_permutation.
@@ -19,7 +19,7 @@ Definition ex_124_permutation: permutation 6.
 Proof.
   refine (let H := (_: permutation_list 6) in plist_to_permutation H).
   pose (5::2::0::1::4::3::nil) as L. exists L. pose (aux3_reflect 6 L).
-  simpl in *. inversion r. auto.
+  inversion r. auto.
 Defined.
 Eval compute in show ex_124_permutation.
 Eval compute in count_inversions ex_124_permutation.
@@ -29,7 +29,7 @@ Definition ex_125_permutation: permutation 9.
 Proof.
   refine (let H := (_: permutation_list 9) in plist_to_permutation H).
   pose (0::8::5::2::1::4::3::6::7::nil) as L. exists L. pose (aux3_reflect 9 L).
-  simpl in *. inversion r. auto.
+  inversion r. auto.
 Defined.
 Eval compute in show ex_125_permutation.
 Eval compute in count_inversions ex_125_permutation.
@@ -39,12 +39,108 @@ Definition ex_126_permutation: permutation 7.
 Proof.
   refine (let H := (_: permutation_list 7) in plist_to_permutation H).
   pose (6::4::5::3::0::2::1::nil) as L. exists L. pose (aux3_reflect 7 L).
-  simpl in *. inversion r. auto.
+  inversion r. auto.
 Defined.
 Eval compute in show ex_126_permutation.
 Eval compute in count_inversions ex_126_permutation.
 
+(* Exercise 169 *)
+Definition ex_169_permutation_1: permutation 4.
+Proof.
+  refine (let H := (_: permutation_list 4) in plist_to_permutation H).
+  pose (3::0::2::1::nil) as L. exists L. pose (aux3_reflect 4 L).
+  inversion r. auto.
+Defined.
+Definition ex_169_permutation_2: permutation 4.
+Proof.
+  refine (let H := (_: permutation_list 4) in plist_to_permutation H).
+  pose (2::1::3::0::nil) as L. exists L. pose (aux3_reflect 4 L).
+  inversion r. auto.
+Defined.
+Definition ex_169_result := permutation_mult ex_169_permutation_1 ex_169_permutation_2.
+Eval compute in show ex_169_permutation_1.
+Eval compute in show ex_169_permutation_2.
+Eval compute in show ex_169_result.
 
+(* Exercise 170 *)
+Definition ex_170_permutation_1: permutation 5.
+Proof.
+  refine (let H := (_: permutation_list 5) in plist_to_permutation H).
+  pose (1::3::4::0::2::nil) as L. exists L. pose (aux3_reflect 5 L).
+  inversion r. auto.
+Defined.
+Definition ex_170_permutation_2: permutation 5.
+Proof.
+  refine (let H := (_: permutation_list 5) in plist_to_permutation H).
+  pose (4::2::3::0::1::nil) as L. exists L. pose (aux3_reflect 5 L).
+  inversion r. auto.
+Defined.
+Definition ex_170_result := permutation_mult ex_170_permutation_1 ex_170_permutation_2.
+Eval compute in show ex_170_permutation_1.
+Eval compute in show ex_170_permutation_2.
+Eval compute in show ex_170_result.
+
+(* Exercise 171 *)
+Definition ex_171_permutation_1: permutation 5.
+Proof.
+  refine (let H := (_: permutation_list 5) in plist_to_permutation H).
+  pose (2::4::0::1::3::nil) as L. exists L. pose (aux3_reflect 5 L).
+  inversion r. auto.
+Defined.
+Definition ex_171_permutation_2: permutation 5.
+Proof.
+  refine (let H := (_: permutation_list 5) in plist_to_permutation H).
+  pose (2::3::0::4::1::nil) as L. exists L. pose (aux3_reflect 5 L).
+  inversion r. auto.
+Defined.
+Definition ex_171_result := permutation_mult ex_171_permutation_1 ex_171_permutation_2.
+Eval compute in show ex_171_permutation_1.
+Eval compute in show ex_171_permutation_2.
+Eval compute in show ex_171_result.
+
+(* Exercise 172 *)
+Definition ex_172_permutation: permutation 4.
+Proof.
+  refine (let H := (_: permutation_list 4) in plist_to_permutation H).
+  pose (1::2::3::0::nil) as L. exists L. pose (aux3_reflect 4 L).
+  inversion r. auto.
+Defined.
+Definition ex_172_result := permutation_power ex_172_permutation 2.
+Eval compute in show ex_172_permutation.
+Eval compute in show ex_172_result.
+
+(* Exercise 173 *)
+Definition ex_173_permutation: permutation 5.
+Proof.
+  refine (let H := (_: permutation_list 5) in plist_to_permutation H).
+  pose (2::3::4::0::1::nil) as L. exists L. pose (aux3_reflect 5 L).
+  inversion r. auto.
+Defined.
+Definition ex_173_result := permutation_power ex_173_permutation 3.
+Eval compute in show ex_173_permutation.
+Eval compute in show ex_173_result.
+
+(* Exercise 176 *)
+Definition ex_176_permutation: permutation 10.
+Proof.
+  refine (let H := (_: permutation_list 10) in plist_to_permutation H).
+  pose (2::4::3::0::6::9::1::5::8::7::nil) as L. exists L. pose (aux3_reflect 10 L).
+  inversion r. auto.
+Defined.
+Definition ex_176_result_naive := permutation_power ex_176_permutation 100.
+Eval compute in show ex_176_permutation.
+Eval compute in show ex_176_result_naive.
+
+(* Exercise 177 *)
+Definition ex_177_permutation: permutation 10.
+Proof.
+  refine (let H := (_: permutation_list 10) in plist_to_permutation H).
+  pose (2::4::3::5::8::6::0::9::7::1::nil) as L. exists L. pose (aux3_reflect 10 L).
+  inversion r. auto.
+Defined.
+Definition ex_177_result_naive := permutation_power ex_177_permutation 150.
+Eval compute in show ex_177_permutation.
+Eval compute in show ex_177_result_naive.
 
 (* Different tests *)
 Definition test_permutation: permutation 3.
